src/Std/Tactic/RSimp/ConvTheorem.lean
@@ -6,6 +6,7 @@ Authors: Joachim Breitner
 
 prelude
 import Std.Tactic.RSimp.Setup
+import Std.Tactic.RSimp.Fuel
 import Lean.Elab.Tactic
 import Lean.Elab.DeclUtil
 import Lean.Elab.Command
@@ -13,22 +14,39 @@ import Lean.Elab.Tactic.Conv
 import Init.Tactics
 import Init.Conv
 
-open Lean.Parser in
-/--
-Abstracts the right-hand side into its own constant of the given name, and
-uses it in the `conv_theorem`.
--/
-def namedRhs := leading_parser
-  atomic (" (" >> nonReservedSymbol "abstract_rhs") >> " := " >> ident >> ")"
-
 open Lean.Parser.Tactic in
 /--
 TODO
 -/
-syntax (name := convTheorem) declModifiers "conv_theorem" (namedRhs)? declId declSig " => " Conv.convSeq : command
+syntax (name := convTheorem) declModifiers "conv_theorem" declId declSig " => " Conv.convSeq : command
 
+open Lean.Parser.Tactic in
+syntax (name := withFuel) "withFuel" " => " Conv.convSeq : conv
 
-open Lean Meta Elab Command Tactic
+syntax (name := abstractAs) "abstractAs " nestedDeclModifiers ident : conv
+
+open Lean Meta Elab Command Tactic Conv
+
+@[tactic withFuel] def evalWithFuel : Tactic := fun stx => do
+  let lhs ← getLhs
+  withMainContext do
+    -- TODO: This needs to generalize some variables first
+    let (rhs, proof) ← convert lhs (evalTactic stx[2])
+    if lhs == rhs then
+      throwError "Non-productive recursive equation {lhs} = {rhs}."
+    else if let some (rhs', proof') ← recursionToFuel? lhs rhs proof then
+      updateLhs rhs' proof'
+    else
+      throwError "Did not find {lhs} in {rhs}."
+
+@[tactic abstractAs] def evalAbstractAs : Tactic := fun stx => do
+  let lhs ← getLhs
+  let modifiers ← elabModifiers ⟨stx[1]⟩
+  let declId := stx[2]
+  let ⟨_, declName, _⟩ ← Term.expandDeclId (← getCurrNamespace) (← Term.getLevelNames) declId modifiers
+  let e ← mkAuxDefinitionFor declName lhs
+  withSaveInfoContext <| Term.addTermInfo' declId e.getAppFn (isBinder := true)
+  changeLhs e
 
 def convert (lhs : Expr) (conv : TacticM Unit) : TermElabM (Expr × Expr) := do
   let (rhs, newGoal) ← Conv.mkConvGoalFor lhs
@@ -44,20 +62,21 @@ def convert (lhs : Expr) (conv : TacticM Unit) : TermElabM (Expr × Expr) := do
 @[command_elab convTheorem]
 def elabConvTheorem : CommandElab := fun stx => do
   let modifiers ← elabModifiers ⟨stx[0]⟩
-  let declId             := stx[3]
-  let (binders, lhsStx) := expandDeclSig stx[4]
-  let scopeLevelNames ← getLevelNames
-  let ⟨_, declName, allUserLevelNames⟩ ← expandDeclId declId modifiers
-  addDeclarationRanges declName modifiers.stx stx
-  runTermElabM fun vars =>
+  let declId            := stx[2]
+  let (binders, lhsStx) := expandDeclSig stx[3]
+  runTermElabM fun vars => do
+    let scopeLevelNames ← Term.getLevelNames
+    let ⟨shortName, declName, allUserLevelNames⟩ ← Term.expandDeclId (← getCurrNamespace) scopeLevelNames declId modifiers
+    addDeclarationRangesForBuiltin declName modifiers.stx stx
+    Term.withAutoBoundImplicitForbiddenPred (fun n => shortName == n) do
     Term.withDeclName declName <| Term.withLevelNames allUserLevelNames <| Term.elabBinders binders.getArgs fun xs => do
       Term.applyAttributesAt declName modifiers.attrs AttributeApplicationTime.beforeElaboration
-      let lhs ← Term.elabTerm lhsStx none
+      let lhs ← Term.elabTermAndSynthesize lhsStx none
       Term.synthesizeSyntheticMVarsNoPostponing
       let lhs ← instantiateMVars lhs
-      let (rhs, value) ← convert lhs (Tactic.evalTactic stx[6])
-      let type ← mkEq lhs rhs
-      let type ← mkForallFVars xs type
+      let (rhs, value) ← convert lhs (Tactic.evalTactic stx[5])
+      let eqType ← mkEq lhs rhs
+      let type ← mkForallFVars xs eqType
       let type ← mkForallFVars vars type
       let type ← Term.levelMVarToParam type
       let value ← mkLambdaFVars xs value
@@ -68,6 +87,7 @@ def elabConvTheorem : CommandElab := fun stx => do
       | Except.ok levelParams =>
         let type ← instantiateMVars type
         let value ← instantiateMVars value
+
         let decl := Declaration.thmDecl {
           name        := declName,
           levelParams := levelParams,
@@ -76,7 +96,7 @@ def elabConvTheorem : CommandElab := fun stx => do
         }
         Term.ensureNoUnassignedMVars decl
         addDecl decl
-        withSaveInfoContext do  -- save new env
+        withSaveInfoContext do
           Term.addTermInfo' declId (← mkConstWithLevelParams declName) (isBinder := true)
         Term.applyAttributesAt declName modifiers.attrs AttributeApplicationTime.afterTypeChecking
         Term.applyAttributesAt declName modifiers.attrs AttributeApplicationTime.afterCompilation
@@ -88,13 +108,60 @@ conv_theorem test : id 1 + 2 =>
   unfold id
   simp
 
-
+/-- info: test : id 1 + 2 = 3 -/
+#guard_msgs in
 #check test
 
-conv_theorem test2  (a b c : Fin 12) : (a + b + c).val =>
-  skip
+conv_theorem test2 (a b c : Fin 12) : (a + b + c).val =>
   simp [Fin.ext_iff, Fin.val_add]
+  abstractAs /-- docstrings possible! -/ test2_rhs
 
+/--
+info: def test2_rhs : Fin 12 → Fin 12 → Fin 12 → Nat :=
+fun a b c => (↑a + ↑b + ↑c) % 12
+-/
+#guard_msgs in
+#print test2_rhs
+
+/-- info: test2 (a b c : Fin 12) : ↑(a + b + c) = test2_rhs a b c -/
+#guard_msgs in
 #check test2
 
--- test2 (a b c : Fin 12) : ↑(a + b + c) = test2_rhs_aux a b c
+/-- error: unknown identifier 'foo' -/
+#guard_msgs in
+conv_theorem bad_elab1 : foo && true => skip
+
+-- TODO: Why does this not abort nicely
+
+/--
+error: unknown identifier 'foo'
+---
+error: (kernel) declaration has metavariables 'bad_elab2'
+-/
+#guard_msgs in
+conv_theorem bad_elab2 : foo true => skip
+
+def fib : Nat → Nat
+  | 0 => 0
+  | 1 => 1
+  | n+2 => fib n + fib (n+1)
+
+conv_theorem fib_optimize : fib =>
+  withFuel =>
+    ext n
+    unfold fib
+    simp [← Nat.add_eq]
+  abstractAs fib.opt
+
+/--
+info: def fib.opt : Nat → Nat :=
+rsimp_iterate fib fun ih n =>
+  match n with
+  | 0 => 0
+  | 1 => 1
+  | n.succ.succ => (ih n).add (ih (n.add 1))
+-/
+#guard_msgs in
+#print fib.opt
+
+def fib' (n : Nat) := (fib n, fib (n+1))
