src/Std/Tactic/RSimp/Fuel.lean
@@ -1,0 +1,32 @@
+import Lean
+
+open Lean Meta
+
+def lots_of_fuel : Nat := 9223372036854775807
+
+def rsimp_iterate {α : Sort u} (x : α) (f : α → α) : α :=
+  Nat.rec x (fun _ ih => f ih) lots_of_fuel
+
+theorem reduce_with_fuel {α : Sort u} {x : α} {f : α → α} (h : x = f x) :
+    x = rsimp_iterate x f := by
+    unfold rsimp_iterate
+    exact Nat.rec rfl (fun _ ih => h.trans (congrArg f ih)) lots_of_fuel
+
+def recursionToFuel? (lhs rhs proof : Expr) : MetaM (Option (Expr × Expr)) := do
+  let f ← kabstract rhs lhs
+  if f.hasLooseBVars then
+    let t ← inferType lhs
+    let u ← getLevel t
+    let f := mkLambda `ih .default t f
+    let rhs' := mkApp3 (.const ``rsimp_iterate [u]) t lhs f
+    let proof' := mkApp4 (.const ``reduce_with_fuel [u]) t lhs f proof
+    return some (rhs', proof')
+  else
+    return none
+
+def recursionToFuel (lhs rhs proof : Expr) : MetaM (Expr × Expr) := do
+  if let some (rhs', proof') ← recursionToFuel? lhs rhs proof then
+    return (rhs', proof')
+  else
+    -- Not (obviously) recursive
+    return (rhs, proof)
